GET RID OF THE SECOND MEMORY STREAM

src/NLustre/MemSemantics.v
@@ -99,17 +99,16 @@ Module Type MEMSEMANTICS
   Definition memory_masked' (k: nat) (rs: cstream) (M Mk: memories) :=
     forall n, count rs n = k -> M n = Mk n.
 
-  Definition mfby (x: ident) (c0: val) (xs: stream value) (M M': memories) (ys: stream value) : Prop :=
+  Definition mfby (x: ident) (c0: val) (xs: stream value) (M: memories) (ys: stream value) : Prop :=
     find_val x (M 0) = Some c0
-    /\ (forall n, find_val x (M (S n)) = find_val x (M' n))
     /\ forall n, match find_val x (M n) with
            | Some mv =>
              match xs n with
              | absent =>
-               find_val x (M' n) = Some mv
+               find_val x (M (S n)) = Some mv
                /\ ys n = absent
              | present v =>
-               find_val x (M' n) = Some v
+               find_val x (M (S n)) = Some v
                /\ ys n = present mv
              end
            | None => False
@@ -129,57 +128,53 @@ Module Type MEMSEMANTICS
     Definition memory_closed_n (M: memories) (eqs: list equation) : Prop :=
       forall n, memory_closed (M n) eqs.
 
-    Inductive msem_equation: stream bool -> history -> memories -> memories -> equation -> Prop :=
+    Inductive msem_equation: stream bool -> history -> memories -> equation -> Prop :=
     | SEqDef:
-        forall bk H M M' x ck xs ce,
+        forall bk H M x ck xs ce,
           sem_var H x xs ->
           sem_caexp bk H ck ce xs ->
-          msem_equation bk H M M' (EqDef x ck ce)
+          msem_equation bk H M (EqDef x ck ce)
     | SEqApp:
-        forall bk H M M' x xs ck f Mx Mx' arg ls xss,
+        forall bk H M x xs ck f Mx arg ls xss,
           hd_error xs = Some x ->
           sub_inst_n x M Mx ->
-          sub_inst_n x M' Mx' ->
           sem_exps bk H arg ls ->
           sem_vars H xs xss ->
 	        sem_clock bk H ck (clock_of ls) ->
-          msem_node f ls Mx Mx' xss ->
-          msem_equation bk H M M' (EqApp xs ck f arg None)
+          msem_node f ls Mx xss ->
+          msem_equation bk H M (EqApp xs ck f arg None)
     | SEqReset:
-        forall bk H M M' x xs ck f Mx Mx' arg y ys rs ls xss,
+        forall bk H M x xs ck f Mx arg y ys rs ls xss,
           hd_error xs = Some x ->
           sub_inst_n x M Mx ->
-          sub_inst_n x M' Mx' ->
           sem_exps bk H arg ls ->
           sem_vars H xs xss ->
           sem_clock bk H ck (clock_of ls) ->
           sem_var H y ys ->
           bools_of ys rs ->
-          (forall k, exists Mk Mk',
-                msem_node f (mask k rs ls) Mk Mk' (mask k rs xss)
-                /\ memory_masked k rs Mx Mk
-                /\ memory_masked' k rs Mx' Mk') ->
-          msem_equation bk H M M' (EqApp xs ck f arg (Some y))
+          (forall k, exists Mk,
+                msem_node f (mask k rs ls) Mk (mask k rs xss)
+                /\ memory_masked k rs Mx Mk) ->
+          msem_equation bk H M (EqApp xs ck f arg (Some y))
     | SEqFby:
-        forall bk H M M' x ck ls xs c0 le,
+        forall bk H M x ck ls xs c0 le,
           sem_aexp bk H ck le ls ->
           sem_var H x xs ->
-          mfby x (sem_const c0) ls M M' xs ->
-          msem_equation bk H M M' (EqFby x ck c0 le)
+          mfby x (sem_const c0) ls M xs ->
+          msem_equation bk H M (EqFby x ck c0 le)
 
     with msem_node:
-           ident -> stream (list value) -> memories -> memories -> stream (list value) -> Prop :=
+           ident -> stream (list value) -> memories -> stream (list value) -> Prop :=
            SNode:
-             forall bk H f xss M M' yss n,
+             forall bk H f xss M yss n,
                bk = clock_of xss ->
                find_node f G = Some n ->
                sem_vars H (map fst n.(n_in)) xss ->
                sem_vars H (map fst n.(n_out)) yss ->
                sem_clocked_vars bk H (idck n.(n_in)) ->
-               Forall (msem_equation bk H M M') n.(n_eqs) ->
+               Forall (msem_equation bk H M) n.(n_eqs) ->
                memory_closed_n M n.(n_eqs) ->
-               memory_closed_n M' n.(n_eqs) ->
-               msem_node f xss M M' yss.
+               msem_node f xss M yss.
 
   End NodeSemantics.
 
@@ -193,87 +188,83 @@ enough: it does not support the internal fixpoint introduced by
 
     Variable G: global.
 
-    Variable P_equation: stream bool -> history -> memories -> memories -> equation -> Prop.
-    Variable P_node: ident -> stream (list value) -> memories -> memories -> stream (list value) -> Prop.
+    Variable P_equation: stream bool -> history -> memories -> equation -> Prop.
+    Variable P_node: ident -> stream (list value) -> memories -> stream (list value) -> Prop.
 
     Hypothesis EqDefCase:
-      forall bk H M M' x ck xs ce,
+      forall bk H M x ck xs ce,
         sem_var H x xs ->
         sem_caexp bk H ck ce xs ->
-        P_equation bk H M M' (EqDef x ck ce).
+        P_equation bk H M (EqDef x ck ce).
 
     Hypothesis EqAppCase:
-      forall bk H M M' x xs ck f Mx Mx' arg ls xss,
+      forall bk H M x xs ck f Mx arg ls xss,
         Some x = hd_error xs ->
         sub_inst_n x M Mx ->
-        sub_inst_n x M' Mx' ->
         sem_exps bk H arg ls ->
         sem_vars H xs xss ->
         sem_clock bk H ck (clock_of ls) ->
-        msem_node G f ls Mx Mx' xss ->
-        P_node f ls Mx Mx' xss ->
-        P_equation bk H M M' (EqApp xs ck f arg None).
+        msem_node G f ls Mx xss ->
+        P_node f ls Mx xss ->
+        P_equation bk H M (EqApp xs ck f arg None).
 
     Hypothesis EqResetCase:
-      forall bk H M M' x xs ck f Mx Mx' arg y ys rs ls xss,
+      forall bk H M x xs ck f Mx arg y ys rs ls xss,
         Some x = hd_error xs ->
         sub_inst_n x M Mx ->
-        sub_inst_n x M' Mx' ->
         sem_exps bk H arg ls ->
         sem_vars H xs xss ->
         sem_clock bk H ck (clock_of ls) ->
         sem_var H y ys ->
         bools_of ys rs ->
-        (forall k, exists Mk Mk',
-              msem_node G f (mask k rs ls) Mk Mk' (mask k rs xss)
+        (forall k, exists Mk,
+              msem_node G f (mask k rs ls) Mk (mask k rs xss)
               /\ memory_masked k rs Mx Mk
-              /\ memory_masked' k rs Mx' Mk'
-              /\ P_node f (mask k rs ls) Mk Mk' (mask k rs xss)) ->
-        P_equation bk H M M' (EqApp xs ck f arg (Some y)).
+              /\ P_node f (mask k rs ls) Mk (mask k rs xss)) ->
+        P_equation bk H M (EqApp xs ck f arg (Some y)).
 
     Hypothesis EqFbyCase:
-      forall bk H M M' x ck ls xs c0 le,
+      forall bk H M x ck ls xs c0 le,
         sem_aexp bk H ck le ls ->
         sem_var H x xs ->
-        mfby x (sem_const c0) ls M M' xs ->
-        P_equation bk H M M' (EqFby x ck c0 le).
+        mfby x (sem_const c0) ls M xs ->
+        P_equation bk H M (EqFby x ck c0 le).
 
     Hypothesis NodeCase:
-      forall bk H f xss M M' yss n,
+      forall bk H f xss M yss n,
         bk = clock_of xss ->
         find_node f G = Some n ->
         sem_vars H (map fst n.(n_in)) xss ->
         sem_vars H (map fst n.(n_out)) yss ->
         sem_clocked_vars bk H (idck n.(n_in)) ->
-        Forall (msem_equation G bk H M M') n.(n_eqs) ->
+        Forall (msem_equation G bk H M) n.(n_eqs) ->
         memory_closed_n M n.(n_eqs) ->
-        memory_closed_n M' n.(n_eqs) ->
-        Forall (P_equation bk H M M') n.(n_eqs) ->
-        P_node f xss M M' yss.
+        Forall (P_equation bk H M) n.(n_eqs) ->
+        P_node f xss M yss.
 
     Fixpoint msem_equation_mult
-             (b: stream bool) (H: history) (M M': memories) (e: equation)
-             (Sem: msem_equation G b H M M' e) {struct Sem}
-      : P_equation b H M M' e
+             (b: stream bool) (H: history) (M: memories) (e: equation)
+             (Sem: msem_equation G b H M e) {struct Sem}
+      : P_equation b H M e
     with msem_node_mult
            (f: ident)
            (xss: stream (list value))
-           (M M': memories)
+           (M: memories)
            (oss: stream (list value))
-           (Sem: msem_node G f xss M M' oss) {struct Sem}
-         : P_node f xss M M' oss.
+           (Sem: msem_node G f xss M oss) {struct Sem}
+         : P_node f xss M oss.
     Proof.
       - destruct Sem; eauto.
         eapply EqResetCase; eauto.
         match goal with
-          H: forall _, exists _ _, _ |- _ =>
-          intro k; destruct (H k) as (?&?&?&?&?); eauto 7
+          H: forall _, exists _, _ |- _ =>
+          intro k; destruct (H k) as (?&?&?); eauto 7
         end.
       - destruct Sem; eauto.
         eapply NodeCase; eauto.
         match goal with
-          H: memory_closed_n M _, H': memory_closed_n M' _, Heqs: Forall _ (n_eqs n)
-          |- _ => clear H H'; induction Heqs; auto
+          H: memory_closed_n M _, Heqs: Forall _ (n_eqs n)
+          |- _ => clear H; induction Heqs; auto
         end.
     Qed.
 
@@ -283,7 +274,7 @@ enough: it does not support the internal fixpoint introduced by
   End msem_node_mult.
 
   Definition msem_nodes (G: global) : Prop :=
-    Forall (fun no => exists xs M M' ys, msem_node G no.(n_name) xs M M' ys) G.
+    Forall (fun no => exists xs M ys, msem_node G no.(n_name) xs M ys) G.
 
 
   (** ** Properties *)
@@ -298,29 +289,29 @@ enough: it does not support the internal fixpoint introduced by
    TODO: try this when the other elements are stabilised. *)
 
   Lemma msem_node_cons:
-    forall n G f xs M M' ys,
+    forall n G f xs M ys,
       Ordered_nodes (n :: G) ->
-      msem_node (n :: G) f xs M M' ys ->
+      msem_node (n :: G) f xs M ys ->
       n.(n_name) <> f ->
-      msem_node G f xs M M' ys.
+      msem_node G f xs M ys.
   Proof.
     Hint Constructors msem_node msem_equation.
     intros * Hord Hsem Hnf.
     revert Hnf.
-    induction Hsem as [| |???????????????????????? Hsems|
-                       |????????? Hf ?????? IH]
+    induction Hsem as [| |????????????????????? Hsems|
+                       |???????? Hf ????? IH]
         using msem_node_mult
-      with (P_equation := fun bk H M M' eq =>
+      with (P_equation := fun bk H M eq =>
                             ~Is_node_in_eq n.(n_name) eq ->
-                            msem_equation G bk H M M' eq);
+                            msem_equation G bk H M eq);
       eauto.
     - intro Hnin.
       econstructor; eauto.
       apply IHHsem. intro; apply Hnin; subst. constructor.
     - intro Hnin.
       econstructor; eauto.
-      intro k; destruct (Hsems k) as (?&?&?&?&?& IH).
-      do 2 eexists; split; eauto.
+      intro k; destruct (Hsems k) as (?&?&?& IH).
+      eexists; split; eauto.
       apply IH; intro; apply Hnin; subst. constructor.
     - intro.
       rewrite find_node_tl with (1:=Hnf) in Hf.
@@ -354,21 +345,21 @@ enough: it does not support the internal fixpoint introduced by
     forall n G,
       Ordered_nodes G ->
       Forall (fun n' => n.(n_name) <> n'.(n_name)) G ->
-      (forall f xv M M' yv,
-          msem_node G f xv M M' yv ->
-          msem_node (n :: G) f xv M M' yv)
+      (forall f xv M yv,
+          msem_node G f xv M yv ->
+          msem_node (n :: G) f xv M yv)
       /\
-      (forall bk R M M' eq,
-          msem_equation G bk R M M' eq ->
+      (forall bk R M eq,
+          msem_equation G bk R M eq ->
           ~Is_node_in_eq n.(n_name) eq ->
-          msem_equation (n::G) bk R M M' eq).
+          msem_equation (n::G) bk R M eq).
   Proof.
     intros n G OG Fn.
     apply msem_node_equation_ind; try (now intros; econstructor; eauto).
     - intros. econstructor; eauto. intro k.
       take (forall k, exists Mr, _) and specialize (it k);
-        destruct it as (Mk & Mk' & ? & ? & ? & ?).
-      exists Mk, Mk'. split; auto.
+        destruct it as (Mk & ? & ? & ?).
+      exists Mk. split; auto.
     - intros.
       take (find_node f G = Some _) and rename it into Ff.
       econstructor; eauto.
@@ -383,19 +374,19 @@ enough: it does not support the internal fixpoint introduced by
   Qed.
 
   Lemma msem_node_cons2:
-    forall n G f xs M M' ys,
+    forall n G f xs M ys,
       Ordered_nodes G ->
-      msem_node G f xs M M' ys ->
+      msem_node G f xs M ys ->
       Forall (fun n' => n_name n <> n_name n') G ->
-      msem_node (n :: G) f xs M M' ys.
+      msem_node (n :: G) f xs M ys.
   Proof. intros; apply msem_cons2; auto. Qed.
 
   Lemma msem_equations_cons:
-    forall G bk H M M' eqs n,
+    forall G bk H M eqs n,
       Ordered_nodes (n :: G) ->
       ~Is_node_in n.(n_name) eqs ->
-      (Forall (msem_equation G bk H M M') eqs <->
-       Forall (msem_equation (n :: G) bk H M M') eqs).
+      (Forall (msem_equation G bk H M) eqs <->
+       Forall (msem_equation (n :: G) bk H M) eqs).
   Proof.
     intros * Hord Hnini.
     induction eqs as [|eq eqs IH]; [now constructor|].
@@ -403,26 +394,26 @@ enough: it does not support the internal fixpoint introduced by
     split; intros Hsem; apply Forall_cons2 in Hsem as [Heq Heqs];
       apply IH in Heqs; auto; constructor; auto.
     - inv Hord.
-      destruct Heq as [| |???????????????????????? Hsems|]; eauto.
+      destruct Heq as [| |????????????????????? Hsems|]; eauto.
       + eauto using msem_node_cons2.
       + econstructor; eauto.
-        intro k; destruct (Hsems k) as (?&?&?&?&?).
-        do 2 eexists; split; eauto using msem_node_cons2.
-    - inversion Heq as [| |???????????????????????? Hsems|]; subst; eauto;
+        intro k; destruct (Hsems k) as (?&?&?).
+        eexists; split; eauto using msem_node_cons2.
+    - inversion Heq as [| |????????????????????? Hsems|]; subst; eauto;
         assert (n.(n_name) <> f)
         by (intro HH; apply Hnini; rewrite HH; constructor).
       + eauto using msem_node_cons.
       + econstructor; eauto.
-        intro k; destruct (Hsems k) as (?&?&?&?&?).
-        do 2 eexists; split; eauto using msem_node_cons.
+        intro k; destruct (Hsems k) as (?&?&?).
+        eexists; split; eauto using msem_node_cons.
   Qed.
 
   Lemma find_node_msem_node:
     forall G f,
       msem_nodes G ->
       find_node f G <> None ->
-      exists xs M M' ys,
-        msem_node G f xs M M' ys.
+      exists xs M ys,
+        msem_node G f xs M ys.
   Proof.
     intros G f Hnds Hfind.
     apply find_node_Exists in Hfind.
@@ -431,8 +422,8 @@ enough: it does not support the internal fixpoint introduced by
     unfold msem_nodes in Hnds.
     rewrite Forall_forall in Hnds.
     apply Hnds in Hin.
-    destruct Hin as [xs [M [M' [ys Hmsem]]]].
-    exists xs, M, M', ys.
+    destruct Hin as [xs [M [ys Hmsem]]].
+    exists xs, M, ys.
     rewrite Hf in *.
     exact Hmsem.
   Qed.
@@ -443,16 +434,15 @@ enough: it does not support the internal fixpoint introduced by
     fun n => add_val y (ms n) (M n).
 
   Lemma mfby_add_val_n:
-    forall x v0 ls M M' xs y ms ms',
+    forall x v0 ls M xs y ms,
       x <> y ->
-      mfby x v0 ls M M' xs ->
-      mfby x v0 ls (add_val_n y ms M) (add_val_n y ms' M') xs.
+      mfby x v0 ls M xs ->
+      mfby x v0 ls (add_val_n y ms M) xs.
   Proof.
     unfold add_val_n.
-    intros * Hxy Fby; destruct Fby as (?&?& Spec).
-    split; [|split].
+    intros * Hxy Fby; destruct Fby as (?& Spec).
+    split.
     - rewrite find_val_gso; auto.
-    - intro; rewrite 2 find_val_gso; auto.
     - intro n; rewrite 2 find_val_gso; auto; apply Spec.
   Qed.
 
@@ -460,9 +450,9 @@ enough: it does not support the internal fixpoint introduced by
     fun n => add_inst y (M' n) (M n).
 
   Lemma mfby_add_inst_n:
-    forall x v0 ls M M' xs y My My',
-      mfby x v0 ls M M' xs ->
-      mfby x v0 ls (add_inst_n y My M) (add_inst_n y My' M') xs.
+    forall x v0 ls M xs y My,
+      mfby x v0 ls M xs ->
+      mfby x v0 ls (add_inst_n y My M) xs.
   Proof.
     inversion 1; econstructor; eauto.
   Qed.
@@ -470,10 +460,10 @@ enough: it does not support the internal fixpoint introduced by
   Hint Resolve mfby_add_val_n mfby_add_inst_n.
 
   Lemma msem_equation_madd_val:
-    forall G bk H M M' x ms ms' eqs,
+    forall G bk H M x ms eqs,
       ~Is_defined_in x eqs ->
-      Forall (msem_equation G bk H M M') eqs ->
-      Forall (msem_equation G bk H (add_val_n x ms M) (add_val_n x ms' M')) eqs.
+      Forall (msem_equation G bk H M) eqs ->
+      Forall (msem_equation G bk H (add_val_n x ms M)) eqs.
   Proof.
     Hint Constructors msem_equation.
     intros * Hnd Hsem.
@@ -489,10 +479,10 @@ enough: it does not support the internal fixpoint introduced by
   Qed.
 
   Lemma msem_equation_madd_inst:
-    forall G bk H M M' Mx Mx' x eqs,
+    forall G bk H M Mx x eqs,
       ~Is_defined_in x eqs ->
-      Forall (msem_equation G bk H M M') eqs ->
-      Forall (msem_equation G bk H (add_inst_n x Mx M) (add_inst_n x Mx' M')) eqs.
+      Forall (msem_equation G bk H M) eqs ->
+      Forall (msem_equation G bk H (add_inst_n x Mx M)) eqs.
   Proof.
     Hint Constructors msem_equation.
     intros * Hnd Hsem.
@@ -502,15 +492,10 @@ enough: it does not support the internal fixpoint introduced by
     apply Forall_cons2 in Hsem.
     destruct Hsem as [Hsem Hsems].
     constructor; [|now apply IH with (1:=Hnds) (2:=Hsems)].
-    destruct Hsem as [|???? x' ???????? Hsome
-                         |???? x' ??????????? Hsome|];
+    destruct Hsem as [|??? x' ??????? Hsome
+                         |??? x' ?????????? Hsome|];
       eauto;
       assert (sub_inst_n x' (add_inst_n x Mx M) Mx0)
-        by (apply not_Is_defined_in_eq_EqApp in Hnd;
-            unfold add_inst_n in *; intro;
-            rewrite find_inst_gso; auto; intro; subst x; destruct xs;
-            inv Hsome; apply Hnd; now constructor);
-      assert (sub_inst_n x' (add_inst_n x Mx' M') Mx'0)
         by (apply not_Is_defined_in_eq_EqApp in Hnd;
             unfold add_inst_n in *; intro;
             rewrite find_inst_gso; auto; intro; subst x; destruct xs;
@@ -603,25 +588,20 @@ dataflow memory for which the non-standard semantics holds true.
     forall G f r xs ys,
       (forall f xs ys,
           sem_node G f xs ys ->
-          exists M M', msem_node G f xs M M' ys) ->
+          exists M, msem_node G f xs M ys) ->
       (forall k, sem_node G f (mask k r xs) (mask k r ys)) ->
-      exists M M',
-      forall k, exists Mk Mk', msem_node G f (mask k r xs) Mk Mk' (mask k r ys)
-                     /\ memory_masked k r M Mk
-                     /\ memory_masked' k r M' Mk'.
+      exists M,
+      forall k, exists Mk, msem_node G f (mask k r xs) Mk (mask k r ys)
+                     /\ memory_masked k r M Mk.
   Proof.
     intros * IH Sem.
-    assert (forall k, exists Mk Mk', msem_node G f (mask k r xs)
-                                     Mk Mk'
-                                     (mask k r ys)) as Msem
+    assert (forall k, exists Mk, msem_node G f (mask k r xs) Mk (mask k r ys)) as Msem
         by (intro; specialize (Sem k); apply IH in Sem; auto).
-    assert (exists F F', forall k, msem_node G f (mask k r xs)
-                                   (F k) (F' k)
-                                   (mask k r ys))
-      as (F & F' & Msem').
+    assert (exists F, forall k, msem_node G f (mask k r xs) (F k) (mask k r ys))
+      as (F & Msem').
     {
       (** Infinite Description  *)
-      do 2 apply functional_choice in Msem as (?& Msem); eauto.
+      apply functional_choice in Msem as (?&?); eauto.
 
       (** Epsilon  *)
       (* assert (inhabited memories) as I *)
@@ -639,7 +619,7 @@ dataflow memory for which the non-standard semantics holds true.
     }
     clear Msem Sem.
 
-    exists (fun n => F (if r n then pred (count r n) else count r n) n), (fun n => F' (count r n) n).
+    exists (fun n => F (if r n then pred (count r n) else count r n) n).
     intro k; specialize (Msem' k).
     do 2 eexists; intuition eauto;
       intros n Count; auto.
@@ -647,31 +627,29 @@ dataflow memory for which the non-standard semantics holds true.
   Qed.
 
   Lemma sem_msem_eq:
-    forall G bk H eqs M M' eq,
+    forall G bk H eqs M eq,
       (forall f xs ys,
           sem_node G f xs ys ->
-          exists M M', msem_node G f xs M M' ys) ->
+          exists M, msem_node G f xs M ys) ->
       sem_equation G bk H eq ->
       NoDup_defs (eq :: eqs) ->
-      Forall (msem_equation G bk H M M') eqs ->
+      Forall (msem_equation G bk H M) eqs ->
       memory_closed_n M eqs ->
-      memory_closed_n M' eqs ->
-      exists M1 M1', Forall (msem_equation G bk H M1 M1') (eq :: eqs)
-                /\ memory_closed_n M1 (eq :: eqs)
-                /\ memory_closed_n M1' (eq :: eqs).
+      exists M1, Forall (msem_equation G bk H M1) (eq :: eqs)
+            /\ memory_closed_n M1 (eq :: eqs).
   Proof.
-    intros * IH Heq NoDup Hmeqs WF WF'.
+    intros * IH Heq NoDup Hmeqs WF.
     inversion Heq as [|
                       ???????? Hls Hxs ? Hsem|
                       ??????????? Hls Hxs ? Hy Hr Hsem|
                       ???????? Hle Hvar Hfby];
       match goal with H:_=eq |- _ => rewrite <-H in * end.
 
-    - exists M, M'.
+    - exists M.
       econstructor; eauto.
 
-    - apply IH in Hsem as (Mx & Mx' & Hmsem).
-      exists (add_inst_n (hd Ids.default x) Mx M), (add_inst_n (hd Ids.default x) Mx' M').
+    - apply IH in Hsem as (Mx & Hmsem).
+      exists (add_inst_n (hd Ids.default x) Mx M).
 
       assert (exists i, hd_error x = Some i) as [i Hsome].
       { assert (Hlen: 0 < length x).
@@ -680,7 +658,7 @@ dataflow memory for which the non-standard semantics holds true.
 
           assert (exists n, length (map fst n.(n_out)) = length (xs 0)
                        /\ 0 < length n.(n_out)) as (n & ? & ?).
-          { inversion_clear Hmsem as [??????????? Out].
+          { inversion_clear Hmsem as [?????????? Out].
             exists n; split; auto.
             - eapply Forall2_length; eauto.
               specialize (Out 0); eauto.
@@ -702,8 +680,8 @@ dataflow memory for which the non-standard semantics holds true.
       + split; apply memory_closed_n_App; auto.
 
     - pose proof Hsem as Hsem'.
-      apply sem_msem_reset in Hsem as (Mx & Mx' & Hmsem); auto.
-      exists (add_inst_n (hd Ids.default x) Mx M), (add_inst_n (hd Ids.default x) Mx' M').
+      apply sem_msem_reset in Hsem as (Mx & Hmsem); auto.
+      exists (add_inst_n (hd Ids.default x) Mx M).
 
       assert (exists i, hd_error x = Some i) as [i Hsome].
       { assert (Hlen: 0 < length x).
@@ -712,8 +690,8 @@ dataflow memory for which the non-standard semantics holds true.
 
           assert (exists n, length (map fst n.(n_out)) = length (xs 0)
                        /\ 0 < length n.(n_out)) as (n & ? & ?).
-          { destruct (Hmsem 0) as (?&?& Hmsem' & ?);
-              inversion_clear Hmsem' as [??????????? Hout].
+          { destruct (Hmsem 0) as (?& Hmsem' & ?);
+              inversion_clear Hmsem' as [?????????? Hout].
             exists n; split; auto.
             - unfold sem_vars, lift in Hout; specialize (Hout 0).
               apply Forall2_length in Hout; rewrite Hout.
@@ -738,15 +716,11 @@ dataflow memory for which the non-standard semantics holds true.
           apply msem_equation_madd_inst; auto.
       + split; apply memory_closed_n_App; auto.
 
-    - exists (add_val_n x (hold (sem_const c0) ls) M), (add_val_n x (fun n =>
-                                                                  match ls n with
-                                                                  | present v => v
-                                                                  | absent => hold (sem_const c0) ls n
-                                                                  end) M');
+    - exists (add_val_n x (hold (sem_const c0) ls) M);
         split.
       + constructor.
         * unfold add_val_n.
-          econstructor; eauto; split; [|split];
+          econstructor; eauto; split;
             intros; try rewrite Hfby; unfold fby;
               simpl; repeat rewrite find_val_gss; auto.
           destruct (ls n); auto.
@@ -769,19 +743,18 @@ dataflow memory for which the non-standard semantics holds true.
     forall G bk H eqs,
       (forall f xs ys,
           sem_node G f xs ys ->
-          exists M M', msem_node G f xs M M' ys) ->
+          exists M, msem_node G f xs M ys) ->
       NoDup_defs eqs ->
       Forall (sem_equation G bk H) eqs ->
-      exists M1 M1', Forall (msem_equation G bk H M1 M1') eqs
-                /\ memory_closed_n M1 eqs
-                /\ memory_closed_n M1' eqs.
+      exists M1, Forall (msem_equation G bk H M1) eqs
+            /\ memory_closed_n M1 eqs.
   Proof.
     intros G bk H eqs IH NoDup Heqs.
     induction eqs as [|eq eqs IHeqs].
-    - exists (fun n => empty_memory _), (fun n => empty_memory _); split; auto.
-      split; apply memory_closed_empty'.
+    - exists (fun n => empty_memory _); split; auto.
+      apply memory_closed_empty'.
     - apply Forall_cons2 in Heqs as [Heq Heqs].
-      eapply IHeqs in Heqs as (?&?&?&?&?).
+      eapply IHeqs in Heqs as (?&?&?).
       + eapply sem_msem_eq; eauto.
       + eapply NoDup_defs_cons; eauto.
   Qed.
@@ -790,7 +763,7 @@ dataflow memory for which the non-standard semantics holds true.
     forall G f xs ys,
       Ordered_nodes G ->
       sem_node G f xs ys ->
-      exists M M', msem_node G f xs M M' ys.
+      exists M, msem_node G f xs M ys.
   Proof.
     induction G as [|node].
     inversion 2;
@@ -808,21 +781,20 @@ dataflow memory for which the non-standard semantics holds true.
       eapply Forall_sem_equation_global_tl in Heqs; eauto.
       assert (forall f xs ys,
                  sem_node G f xs ys ->
-                 exists M M', msem_node G f xs M M' ys) as IHG'
+                 exists M, msem_node G f xs M ys) as IHG'
           by auto.
-      assert (exists M1 M1', Forall (msem_equation G (clock_of xs) H M1 M1') n.(n_eqs)
-                        /\ memory_closed_n M1 n.(n_eqs)
-                        /\ memory_closed_n M1' n.(n_eqs))
-        as (M1 & M1' & Hmsem & ?&?)
+      assert (exists M1, Forall (msem_equation G (clock_of xs) H M1) n.(n_eqs)
+                    /\ memory_closed_n M1 n.(n_eqs))
+        as (M1 & Hmsem &?)
           by (eapply sem_msem_eqs; eauto; apply NoDup_defs_node).
-      exists M1, M1'.
+      exists M1.
       econstructor; eauto.
       rewrite <-msem_equations_cons; eauto.
     - apply ident_eqb_neq in Hnf.
       apply sem_node_cons with (1:=Hord) (3:=Hnf) in Hsem.
       inv Hord.
-      eapply IHG in Hsem as (M & M' &?); eauto.
-      exists M, M'.
+      eapply IHG in Hsem as (M &?); eauto.
+      exists M.
       now eapply msem_node_cons2; eauto.
   Qed.
 
@@ -852,10 +824,10 @@ dataflow memory for which the non-standard semantics holds true.
     fun n => remove_val x (M n).
 
   Lemma msem_equation_remove_inst:
-    forall G bk eqs H M M' x,
+    forall G bk eqs H M x,
       ~Is_defined_in x eqs ->
-      Forall (msem_equation G bk H M M') eqs ->
-      Forall (msem_equation G bk H (remove_inst_n x M) (remove_inst_n x M')) eqs.
+      Forall (msem_equation G bk H M) eqs ->
+      Forall (msem_equation G bk H (remove_inst_n x M)) eqs.
   Proof.
     Ltac foo H := unfold sub_inst_n in *; intro n;
                 setoid_rewrite find_inst_gro; auto;
@@ -870,20 +842,20 @@ dataflow memory for which the non-standard semantics holds true.
   Qed.
 
   Lemma msem_equation_remove_val:
-    forall G bk eqs H M M' x,
+    forall G bk eqs H M x,
       ~Is_defined_in x eqs ->
-      Forall (msem_equation G bk H M M') eqs ->
-      Forall (msem_equation G bk H (remove_val_n x M) (remove_val_n x M')) eqs.
+      Forall (msem_equation G bk H M) eqs ->
+      Forall (msem_equation G bk H (remove_val_n x M)) eqs.
   Proof.
     induction eqs as [|[]]; intros * Hnotin Sems;
       inversion_clear Sems as [|?? Sem]; auto;
-        inversion_clear Sem as [| | |???????????? Mfby];
+        inversion_clear Sem as [| | |??????????? Mfby];
         apply not_Is_defined_in_cons in Hnotin as (Hnotin &?);
         constructor; eauto using msem_equation.
     assert (x <> i) by (intro E; subst; apply Hnotin; constructor).
-    destruct Mfby as (?&?& Spec).
+    destruct Mfby as (?& Spec).
     econstructor; eauto; unfold remove_val_n.
-    split; [|split]; intros; repeat rewrite find_val_gro; auto.
+    split; intros; repeat rewrite find_val_gro; auto.
     apply Spec.
   Qed.
 
@@ -928,29 +900,29 @@ dataflow memory for which the non-standard semantics holds true.
   Qed.
 
   Lemma msem_eqs_same_initial_memory:
-    forall M1 M1' G eqs bk1 H1 M2 M2' bk2 H2,
-      (forall f xss1 M1 M1' yss1 xss2 M2 M2' yss2,
-          msem_node G f xss1 M1 M1' yss1 ->
-          msem_node G f xss2 M2 M2' yss2 ->
+    forall M1 G eqs bk1 H1 M2 bk2 H2,
+      (forall f xss1 M1 yss1 xss2 M2 yss2,
+          msem_node G f xss1 M1 yss1 ->
+          msem_node G f xss2 M2 yss2 ->
           M1 0 ≋ M2 0) ->
       NoDup_defs eqs ->
       memory_closed_n M1 eqs ->
       memory_closed_n M2 eqs ->
-      Forall (msem_equation G bk1 H1 M1 M1') eqs ->
-      Forall (msem_equation G bk2 H2 M2 M2') eqs ->
+      Forall (msem_equation G bk1 H1 M1) eqs ->
+      Forall (msem_equation G bk2 H2 M2) eqs ->
       M1 0 ≋ M2 0.
   Proof.
     intros * IH Nodup Closed1 Closed2 Heqs1 Heqs2.
-    revert dependent M1; revert dependent M2; revert M1' M2'.
+    revert dependent M1; revert dependent M2.
     induction eqs as [|[] ? IHeqs]; intros;
       inversion_clear Heqs1 as [|?? Sem1 Sems1];
       inversion_clear Heqs2 as [|?? Sem2 Sems2];
-      try inversion Sem1 as [|????????????? Hd1 ????? Node|
-                             ???????????????? Hd1 ?? Args1 ?? Var ? Reset1|
-                             ?????????? Arg1 ? Mfby1];
-      try inversion Sem2 as [|????????????? Hd2|
-                             ???????????????? Hd2 ?? Args2 ???? Reset2|
-                             ?????????? Arg2 ? Mfby2];
+      try inversion Sem1 as [|??????????? Hd1 ???? Node|
+                             ?????????????? Hd1 ?? Args1 ? Var ? Reset1|
+                             ????????? Arg1 ? Mfby1];
+      try inversion Sem2 as [|??????????? Hd2|
+                             ?????????????? Hd2 ?? Args2 ??? Reset2|
+                             ????????? Arg2 ? Mfby2];
       inv Nodup; subst; try discriminate; eauto.
     - assert (forall n, M1 n ≋ empty_memory _) as ->
           by (intro; apply memory_closed_empty; auto).
@@ -981,9 +953,9 @@ dataflow memory for which the non-standard semantics holds true.
         symmetry; erewrite add_remove_inst_same; eauto.
       rewrite Sems1.
       destruct (Reset1 (if rs 0 then pred (count rs 0) else count rs 0))
-        as (M01 &?& Node1 & MemMask1 &?),
+        as (M01 & Node1 & MemMask1),
            (Reset2 (if rs0 0 then pred (count rs0 0) else count rs0 0))
-          as (M02 &?&?& MemMask2 &?).
+          as (M02 &?& MemMask2).
       eapply IH in Node1; eauto.
       rewrite MemMask1, MemMask2, Node1; try reflexivity; simpl; cases.
 
@@ -997,10 +969,10 @@ dataflow memory for which the non-standard semantics holds true.
   Qed.
 
   Theorem same_initial_memory:
-    forall G f xss1 xss2 M1 M2 M1' M2' yss1 yss2,
+    forall G f xss1 xss2 M1 M2 yss1 yss2,
       Ordered_nodes G ->
-      msem_node G f xss1 M1 M1' yss1 ->
-      msem_node G f xss2 M2 M2' yss2 ->
+      msem_node G f xss1 M1 yss1 ->
+      msem_node G f xss2 M2 yss2 ->
       M1 0 ≋ M2 0.
   Proof.
     induction G as [|node].
@@ -1008,8 +980,8 @@ dataflow memory for which the non-standard semantics holds true.
       match goal with Hf: find_node _ [] = _ |- _ => inversion Hf end.
     intros * Hord Hsem1 Hsem2.
     assert (Hsem1' := Hsem1);  assert (Hsem2' := Hsem2).
-    inversion_clear Hsem1' as [???????? Clock1 Hfind1 Ins1 ?? Heqs1];
-      inversion_clear Hsem2' as [???????? Clock2 Hfind2 Ins2 ?? Heqs2].
+    inversion_clear Hsem1' as [??????? Clock1 Hfind1 Ins1 ?? Heqs1];
+      inversion_clear Hsem2' as [??????? Clock2 Hfind2 Ins2 ?? Heqs2].
     rewrite Hfind2 in Hfind1; inv Hfind1.
     pose proof Hord; inv Hord.
     pose proof Hfind2.
@@ -1029,25 +1001,24 @@ dataflow memory for which the non-standard semantics holds true.
   (** Absent Until *)
 
   Lemma mfby_absent_until:
-    forall n0 x v0 ls M M' xs,
-      mfby x v0 ls M M' xs ->
+    forall n0 x v0 ls M xs,
+      mfby x v0 ls M xs ->
       (forall n, n < n0 -> ls n = absent) ->
       forall n, n <= n0 -> find_val x (M n) = Some v0.
   Proof.
     intros * Mfby Abs n E; induction n;
-      destruct Mfby as (Init & Spec & Spec'); auto.
-    rewrite Spec.
-    specialize (Spec' n).
+      destruct Mfby as (Init & Spec); auto.
+    specialize (Spec n).
     destruct (find_val x (M n)); try contradiction.
-    rewrite Abs in Spec'; try omega.
-    destruct Spec' as [->].
+    rewrite Abs in Spec; try omega.
+    destruct Spec as [->].
     apply IHn; omega.
   Qed.
 
   Lemma msem_eqs_absent_until:
-    forall M M' G n0 eqs bk H n,
-    (forall f xss M M' yss,
-        msem_node G f xss M M' yss ->
+    forall M G n0 eqs bk H n,
+    (forall f xss M yss,
+        msem_node G f xss M yss ->
         (forall n, n < n0 -> absent_list (xss n)) ->
         forall n, n <= n0 -> M n ≋ M 0) ->
     Ordered_nodes G ->
@@ -1055,16 +1026,16 @@ dataflow memory for which the non-standard semantics holds true.
     (forall n, n < n0 -> bk n = false) ->
     NoDup_defs eqs ->
     memory_closed_n M eqs ->
-    Forall (msem_equation G bk H M M') eqs ->
+    Forall (msem_equation G bk H M) eqs ->
     M n ≋ M 0.
   Proof.
     intros * IH Hord Spec Absbk Nodup Closed Heqs.
-    revert dependent M; revert dependent M'.
+    revert dependent M.
     induction eqs as [|[] ? IHeqs]; intros;
       inversion_clear Heqs as [|?? Sem Sems];
-      try inversion_clear Sem as [|????????????? Hd ???? Hck Node|
-                                  ???????????????? Hd ???? Hck ?? Reset|
-                                  ?????????? Arg ? Mfby];
+      try inversion_clear Sem as [|??????????? Hd ??? Hck Node|
+                                  ?????????????? Hd ??? Hck ?? Reset|
+                                  ????????? Arg ? Mfby];
       inv Nodup; eauto.
     - assert (forall n, M n ≋ empty_memory _) as E
           by (intro; apply memory_closed_empty; auto).
@@ -1087,9 +1058,9 @@ dataflow memory for which the non-standard semantics holds true.
     - apply msem_equation_remove_inst with (x := x) in Sems.
       + apply IHeqs in Sems; auto.
         *{ destruct (Reset (if rs n then pred (count rs n) else count rs n))
-             as (Mn &?& Node_n & MemMask_n & MemMask_n'),
+             as (Mn & Node_n & MemMask_n),
                 (Reset (if rs 0 then pred (count rs 0) else count rs 0))
-               as (M0 &?&?& MemMask_0 &?).
+               as (M0 &?& MemMask_0).
            assert (Mn 0 ≋ M0 0) as E by (eapply same_initial_memory; eauto).
            apply IH with (n := n) in Node_n; auto.
            - erewrite add_remove_inst_same; eauto;
@@ -1116,7 +1087,7 @@ dataflow memory for which the non-standard semantics holds true.
           inversion_clear Arg as [???? SClock|]; auto.
           contradict SClock; apply not_subrate_clock.
         }
-        destruct Mfby as (Init & Loop & Spec').
+        destruct Mfby as (Init & Spec').
         erewrite add_remove_val_same; eauto;
           symmetry; erewrite add_remove_val_same; eauto.
         now rewrite Sems.
@@ -1124,9 +1095,9 @@ dataflow memory for which the non-standard semantics holds true.
   Qed.
 
   Theorem msem_node_absent_until:
-    forall n0 G f xss M M' yss,
+    forall n0 G f xss M yss,
       Ordered_nodes G ->
-      msem_node G f xss M M' yss ->
+      msem_node G f xss M yss ->
       (forall n, n < n0 -> absent_list (xss n)) ->
       forall n, n <= n0 -> M n ≋ M 0.
   Proof.
@@ -1135,7 +1106,7 @@ dataflow memory for which the non-standard semantics holds true.
       match goal with Hf: find_node _ [] = _ |- _ => inversion Hf end.
     intros * Hord Hsem Abs n Spec.
     assert (Hsem' := Hsem).
-    inversion_clear Hsem' as [???????? Clock Hfind Ins ?? Heqs].
+    inversion_clear Hsem' as [??????? Clock Hfind Ins ?? Heqs].
     assert (forall n, n < n0 -> bk n = false) as Absbk.
     { intros k Spec'; apply Abs in Spec'.
       rewrite Clock.
@@ -1157,50 +1128,47 @@ dataflow memory for which the non-standard semantics holds true.
   (** Absent  *)
 
   Lemma mfby_absent:
-    forall n x v0 ls M M' xs,
-      mfby x v0 ls M M' xs ->
+    forall n x v0 ls M xs,
+      mfby x v0 ls M xs ->
       ls n = absent ->
-      find_val x (M' n) = find_val x (M n).
+      find_val x (M (S n)) = find_val x (M n).
   Proof.
     induction n; intros * Mfby Abs;
-      destruct Mfby as (Init & Spec & Spec').
-    - specialize (Spec' 0); rewrite Init, Abs in Spec'.
+      destruct Mfby as (Init & Spec).
+    - specialize (Spec 0); rewrite Init, Abs in Spec.
       intuition; congruence.
-    - specialize (Spec' (S n)).
+    - specialize (Spec (S n)).
       destruct (find_val x (M (S n))); try contradiction.
-      rewrite Abs in Spec'.
+      rewrite Abs in Spec.
       intuition.
   Qed.
 
   Lemma msem_eqs_absent:
-    forall M M' G eqs bk H vars n,
-    (forall f xss M M' yss n,
-        msem_node G f xss M M' yss ->
+    forall M G eqs bk H vars n,
+    (forall f xss M yss n,
+        msem_node G f xss M yss ->
         absent_list (xss n) ->
-        M' n ≋ M n) ->
+        M (S n) ≋ M n) ->
     Ordered_nodes G ->
     Forall (wc_equation G vars) eqs ->
     Forall (clock_match bk H) vars ->
     bk n = false ->
     NoDup_defs eqs ->
     memory_closed_n M eqs ->
-    memory_closed_n M' eqs ->
-    Forall (msem_equation G bk H M M') eqs ->
-    M' n ≋ M n.
+    Forall (msem_equation G bk H M) eqs ->
+    M (S n) ≋ M n.
   Proof.
-    intros * IH Hord WC ClkM Absbk Nodup Closed Closed' Heqs.
-    revert dependent M; revert dependent M'.
+    intros * IH Hord WC ClkM Absbk Nodup Closed Heqs.
+    revert dependent M.
     induction eqs as [|[] ? IHeqs]; intros;
       inversion_clear Heqs as [|?? Sem Sems];
-      try inversion Sem as [|????????????? Hd ???? Hck Node|
-                            ???????????????? Hd ?? Args ? Hck Var Rst Reset|
-                            ?????????? Arg ? Mfby]; subst;
+      try inversion Sem as [|??????????? Hd ??? Hck Node|
+                            ?????????????? Hd ?? Args Hck Var Rst Reset|
+                            ????????? Arg ? Mfby]; subst;
       inv Nodup; inversion_clear WC as [|?? WC_eq]; eauto.
     - assert (forall n, M n ≋ empty_memory _) as E
           by (intro; apply memory_closed_empty; auto).
-     assert (forall n, M' n ≋ empty_memory _) as E'
-          by (intro; apply memory_closed_empty; auto).
-     rewrite E, E'; reflexivity.
+     rewrite 2 E; reflexivity.
 
     - apply msem_equation_remove_inst with (x := x) in Sems.
       + apply IHeqs in Sems; try eapply memory_closed_n_App'; eauto.
@@ -1215,11 +1183,12 @@ dataflow memory for which the non-standard semantics holds true.
     - apply msem_equation_remove_inst with (x := x) in Sems.
       + apply IHeqs in Sems; try eapply memory_closed_n_App'; eauto.
         destruct (Reset (count rs n))
-          as (Mn & Mn' & Node_n & MemMask_n & MemMask_n').
+          as (Mn & Node_n & MemMask_n).
         erewrite add_remove_inst_same; eauto;
           symmetry; rewrite add_remove_inst_same; eauto.
         rewrite Sems.
-        specialize (MemMask_n' n); specialize (MemMask_n n).
+        pose proof (MemMask_n (S n)) as MemMask_Sn.
+        specialize (MemMask_n n).
         destruct (rs n) eqn: Hr.
         *{ inversion_clear WC_eq as [|???????? WC_reset|].
            assert (In (y, c) vars) as Hin by auto.
@@ -1233,7 +1202,7 @@ dataflow memory for which the non-standard semantics holds true.
              rewrite Absbk; apply not_subrate_clock.
          }
         *{ apply IH with (n := n) in Node_n; auto.
-           - rewrite MemMask_n, MemMask_n', Node_n; auto; reflexivity.
+           - rewrite MemMask_n, MemMask_Sn, Node_n; auto; reflexivity.
            - specialize (Hck n); rewrite Absbk in Hck.
              apply absent_list_mask; try apply all_absent_spec.
              eapply clock_of_instant_false, not_subrate_clock_impl; eauto.
@@ -1242,16 +1211,16 @@ dataflow memory for which the non-standard semantics holds true.
 
     - apply msem_equation_remove_val with (x := i) in Sems; auto.
       apply IHeqs in Sems; try eapply memory_closed_n_Fby'; eauto.
-      assert (find_val i (M' n) = find_val i (M n)) as E.
+      assert (find_val i (M (S n)) = find_val i (M n)) as E.
       { eapply mfby_absent; eauto.
         specialize (Arg n); simpl in Arg.
         rewrite Absbk in Arg.
         inversion_clear Arg as [???? SClock|]; auto.
         contradict SClock; apply not_subrate_clock.
       }
-      destruct Mfby as (Init & Loop & Spec').
-      specialize (Spec' n).
-      destruct (find_val i (M' n)) eqn: Eq', (find_val i (M n)) eqn: Eq;
+      destruct Mfby as (Init & Spec).
+      specialize (Spec n).
+      destruct (find_val i (M (S n))) eqn: Eq', (find_val i (M n)) eqn: Eq;
         try contradiction; inv E.
       erewrite add_remove_val_same; eauto;
         symmetry; erewrite add_remove_val_same; eauto.
@@ -1263,8 +1232,8 @@ dataflow memory for which the non-standard semantics holds true.
     forall G,
       Ordered_nodes G ->
       wc_global G ->
-      (forall f xss M M' yss,
-          msem_node G f xss M M' yss ->
+      (forall f xss M yss,
+          msem_node G f xss M yss ->
           forall bk H n,
             find_node f G = Some n ->
             bk = clock_of xss ->
@@ -1273,8 +1242,8 @@ dataflow memory for which the non-standard semantics holds true.
             Forall (clock_match bk H) (idck n.(n_in)) ->
             Forall (clock_match bk H) (idck n.(n_out)))
       /\
-      (forall bk H M M' eq,
-          msem_equation G bk H M M' eq ->
+      (forall bk H M eq,
+          msem_equation G bk H M eq ->
           forall iface x ck,
             NoDupMembers iface ->
             wc_equation G iface eq ->
@@ -1283,11 +1252,11 @@ dataflow memory for which the non-standard semantics holds true.
             clock_match bk H (x, ck)).
   Proof.
     intros * Hord WCG; apply msem_node_equation_ind;
-      [intros ???????? Hvar Hexp|
-       intros ???????????????? Hexps Hvars Hck Hsem|
-       intros ??????????????????? Hexps Hvars Hck ?? Hsem|
-       intros ?????????? Hexp Hvar Hfby|
-       intros ???????? Hck Hf Hin Hout ???? IH].
+      [intros ??????? Hvar Hexp|
+       intros ????????????? Hexps Hvars Hck Hsem|
+       intros ???????????????? Hexps Hvars Hck ?? Hsem|
+       intros ????????? Hexp Hvar Hfby|
+       intros ??????? Hck Hf Hin Hout ??? IH].
 
     - (* EqDef *)
       intros iface y yck Hnd Hwc Hdef Hin n.
@@ -1301,7 +1270,7 @@ dataflow memory for which the non-standard semantics holds true.
     - (* EqApp *)
       intros IHHsem iface z zck Hndup Hwc Hdef Hiface.
       inversion_clear Hdef as [|? ? ? ? ? Hyys|].
-      inversion_clear Hsem as [cks' H' ????? node Hco' Hfind Hvi Hvo].
+      inversion_clear Hsem as [cks' H' ???? node Hco' Hfind Hvi Hvo].
       specialize (IHHsem _ _ _ Hfind Hco' Hvi Hvo).
       assert (Hvi' := Hvi).
       rewrite <-map_fst_idck in Hvi'.
@@ -1365,9 +1334,9 @@ dataflow memory for which the non-standard semantics holds true.
     - (* EqReset *)
       intros iface z zck Hndup Hwc Hdef Hiface n.
       inversion_clear Hdef as [|? ? ? ? ? Hyys|].
-      specialize (Hsem (count rs n)); destruct Hsem as (?&?& Hsems &?&?& IHHsem).
+      specialize (Hsem (count rs n)); destruct Hsem as (?& Hsems &?& IHHsem).
 
-      inversion_clear Hsems as [cks' H' ????? node Hco' Hfind Hvi Hvo].
+      inversion_clear Hsems as [cks' H' ???? node Hco' Hfind Hvi Hvo].
       specialize (IHHsem _ _ _ Hfind Hco' Hvi Hvo).
       assert (Hvi' := Hvi).
       rewrite <-map_fst_idck in Hvi'.
@@ -1440,7 +1409,7 @@ dataflow memory for which the non-standard semantics holds true.
       inv Hdef; inv Hwc.
       match goal with H1:In (?y, _) iface, H2:In (?y, _) iface |- _ =>
                       apply NoDupMembers_det with (1:=Hnd) (2:=H1) in H2; subst end.
-      destruct Hfby as (Init & Loop & Spec).
+      destruct Hfby as (Init & Spec).
       specialize (Hexp n); specialize (Hvar n); specialize (Spec n).
       destruct (find_val x (M n)) eqn: Find; try contradiction.
       unfold clock_match_instant.
@@ -1493,10 +1462,10 @@ dataflow memory for which the non-standard semantics holds true.
   Qed.
 
   Corollary clock_match_msem_node:
-    forall G f xss M M' yss bk H n,
+    forall G f xss M yss bk H n,
       Ordered_nodes G ->
       wc_global G ->
-      msem_node G f xss M M' yss ->
+      msem_node G f xss M yss ->
       find_node f G = Some n ->
       bk = clock_of xss ->
       sem_vars H (map fst n.(n_in)) xss ->
@@ -1504,38 +1473,38 @@ dataflow memory for which the non-standard semantics holds true.
       Forall (clock_match bk H) (idck n.(n_in)) ->
       Forall (clock_match bk H) (idck n.(n_out)).
   Proof.
-    intros ????????? Ord WCG; intros.
+    intros ???????? Ord WCG; intros.
     eapply (proj1 (clock_match_msem_node_eqs_reset Ord WCG)); eauto.
   Qed.
 
   Corollary clock_match_msem_eq:
-    forall G bk H M M' iface x ck eq,
+    forall G bk H M iface x ck eq,
       Ordered_nodes G ->
       wc_global G ->
       NoDupMembers iface ->
-      msem_equation G bk H M M' eq ->
+      msem_equation G bk H M eq ->
       wc_equation G iface eq ->
       Is_defined_in_eq x eq ->
       In (x, ck) iface ->
       clock_match bk H (x, ck).
   Proof.
-    intros ????????? Ord WCG; intros.
+    intros ???????? Ord WCG; intros.
     eapply (proj2 (clock_match_msem_node_eqs_reset Ord WCG)); eauto.
   Qed.
 
   Corollary clock_match_msem_eqs:
-    forall G bk H M M' inputs vars eqs,
+    forall G bk H M inputs vars eqs,
       Ordered_nodes G ->
       wc_global G ->
       NoDupMembers (inputs ++ vars) ->
-      Forall (msem_equation G bk H M M') eqs ->
+      Forall (msem_equation G bk H M) eqs ->
       Forall (wc_equation G (inputs ++ vars)) eqs ->
       Permutation.Permutation (vars_defined eqs) (map fst vars) ->
       forall x xck,
         In (x, xck) vars ->
         clock_match bk H (x, xck).
   Proof.
-    intros G bk H M M' inputs vars eqs OG WCG Hndup Hsem Hwc Hdef x xck Hin.
+    intros G bk H M inputs vars eqs OG WCG Hndup Hsem Hwc Hdef x xck Hin.
     assert (In x (vars_defined eqs)) as Hxin
         by (now rewrite Hdef; apply in_map with (f:=fst) in Hin).
     apply Is_defined_in_vars_defined, Is_defined_in_In in Hxin
@@ -1547,19 +1516,19 @@ dataflow memory for which the non-standard semantics holds true.
   Qed.
 
   Theorem msem_node_absent:
-    forall G f xss M M' yss n,
+    forall G f xss M yss n,
       Ordered_nodes G ->
       wc_global G ->
-      msem_node G f xss M M' yss ->
+      msem_node G f xss M yss ->
       absent_list (xss n) ->
-      M' n ≋ M n.
+      M (S n) ≋ M n.
   Proof.
     induction G as [|node].
     inversion 3;
       match goal with Hf: find_node _ [] = _ |- _ => inversion Hf end.
     intros * Hord WC Hsem Abs.
     assert (Hsem' := Hsem).
-    inversion_clear Hsem' as [???????? Clock Hfind Ins ?? Heqs].
+    inversion_clear Hsem' as [??????? Clock Hfind Ins ?? Heqs].
     assert (bk n = false) as Absbk
         by (rewrite Clock; unfold nequiv_decb;
             apply existsb_Forall_neg, absent_list_spec_b; auto).
@@ -1590,120 +1559,119 @@ dataflow memory for which the non-standard semantics holds true.
 
   (** Relooper for free *)
 
-  Lemma msem_eqs_relooper:
-    forall M M' G eqs bk H,
-      (forall f xss M M' yss,
-          msem_node G f xss M M' yss ->
-          forall n, M (S n) ≋ M' n) ->
-      Ordered_nodes G ->
-      NoDup_defs eqs ->
-      memory_closed_n M eqs ->
-      memory_closed_n M' eqs ->
-      Forall (msem_equation G bk H M M') eqs ->
-      forall n, M (S n) ≋ M' n.
-  Proof.
-    intros * IH Hord Nodup Closed Closed' Heqs n.
-    revert dependent M; revert dependent M'.
-    induction eqs as [|[] ? IHeqs]; intros;
-      inversion_clear Heqs as [|?? Sem Sems];
-      try inversion Sem as [|????????????? Hd ?? Args ?? Node|
-                            ???????????????? Hd ?? Args ?? Var Rst Reset|
-                            ?????????? Arg ? Mfby]; subst;
-      inv Nodup; eauto.
-    - assert (forall n, M n ≋ empty_memory _) as E
-          by (intro; apply memory_closed_empty; auto).
-     assert (forall n, M' n ≋ empty_memory _) as E'
-          by (intro; apply memory_closed_empty; auto).
-     rewrite E, E'; reflexivity.
+  (* Lemma msem_eqs_relooper: *)
+  (*   forall M G eqs bk H, *)
+  (*     (forall f xss M yss, *)
+  (*         msem_node G f xss M yss -> *)
+  (*         forall n, M (S n) ≋ n) -> *)
+  (*     Ordered_nodes G -> *)
+  (*     NoDup_defs eqs -> *)
+  (*     memory_closed_n M eqs -> *)
+  (*     memory_closed_n eqs -> *)
+  (*     Forall (msem_equation G bk H M M') eqs -> *)
+  (*     forall n, M (S n) ≋ n. *)
+  (* Proof. *)
+  (*   intros * IH Hord Nodup Closed Closed' Heqs n. *)
+  (*   revert dependent M; revert dependent M'. *)
+  (*   induction eqs as [|[] ? IHeqs]; intros; *)
+  (*     inversion_clear Heqs as [|?? Sem Sems]; *)
+  (*     try inversion Sem as [|????????????? Hd ?? Args ?? Node| *)
+  (*                           ???????????????? Hd ?? Args ?? Var Rst Reset| *)
+  (*                           ?????????? Arg ? Mfby]; subst; *)
+  (*     inv Nodup; eauto. *)
+  (*   - assert (forall n, M n ≋ empty_memory _) as E *)
+  (*         by (intro; apply memory_closed_empty; auto). *)
+  (*    assert (forall n, n ≋ empty_memory _) as E' *)
+  (*         by (intro; apply memory_closed_empty; auto). *)
+  (*    rewrite E, E'; reflexivity. *)
 
-    - apply msem_equation_remove_inst with (x := x) in Sems.
-      + apply IHeqs in Sems; try eapply memory_closed_n_App'; eauto.
-        apply IH with (n := n) in Node; auto.
-        erewrite add_remove_inst_same; eauto;
-          symmetry; erewrite add_remove_inst_same; eauto.
-        now rewrite Sems, Node.
-      + apply hd_error_Some_In in Hd; auto.
+  (*   - apply msem_equation_remove_inst with (x := x) in Sems. *)
+  (*     + apply IHeqs in Sems; try eapply memory_closed_n_App'; eauto. *)
+  (*       apply IH with (n := n) in Node; auto. *)
+  (*       erewrite add_remove_inst_same; eauto; *)
+  (*         symmetry; erewrite add_remove_inst_same; eauto. *)
+  (*       now rewrite Sems, Node. *)
+  (*     + apply hd_error_Some_In in Hd; auto. *)
 
-    - apply msem_equation_remove_inst with (x := x) in Sems.
-      + apply IHeqs in Sems; try eapply memory_closed_n_App'; eauto.
-        erewrite add_remove_inst_same; eauto;
-          symmetry; rewrite add_remove_inst_same; eauto.
-        destruct (Reset (count rs n))
-          as (Mn & Mn' & Node_n & MemMask_n & MemMask_n').
-        apply IH with (n := n) in Node_n.
-        rewrite Sems, (MemMask_n' n), (MemMask_n (S n)), Node_n; auto; reflexivity.
-      + apply hd_error_Some_In in Hd; auto.
+  (*   - apply msem_equation_remove_inst with (x := x) in Sems. *)
+  (*     + apply IHeqs in Sems; try eapply memory_closed_n_App'; eauto. *)
+  (*       erewrite add_remove_inst_same; eauto; *)
+  (*         symmetry; rewrite add_remove_inst_same; eauto. *)
+  (*       destruct (Reset (count rs n)) *)
+  (*         as (Mn & Mn' & Node_n & MemMask_n & MemMask_n'). *)
+  (*       apply IH with (n := n) in Node_n. *)
+  (*       rewrite Sems, (MemMask_n' n), (MemMask_n (S n)), Node_n; auto; reflexivity. *)
+  (*     + apply hd_error_Some_In in Hd; auto. *)
 
-    - apply msem_equation_remove_val with (x := i) in Sems; auto.
-      apply IHeqs in Sems; try eapply memory_closed_n_Fby'; eauto.
-      destruct Mfby as (Init & Loop & Spec').
-      specialize (Spec' (S n)).
-      destruct (find_val i (M (S n))) eqn: Eq; try contradiction.
-      erewrite add_remove_val_same; eauto.
-      rewrite Loop in Eq.
-      symmetry; erewrite add_remove_val_same; eauto.
-      now rewrite Sems.
-  Qed.
+  (*   - apply msem_equation_remove_val with (x := i) in Sems; auto. *)
+  (*     apply IHeqs in Sems; try eapply memory_closed_n_Fby'; eauto. *)
+  (*     destruct Mfby as (Init & Loop & Spec'). *)
+  (*     specialize (Spec' (S n)). *)
+  (*     destruct (find_val i (M (S n))) eqn: Eq; try contradiction. *)
+  (*     erewrite add_remove_val_same; eauto. *)
+  (*     rewrite Loop in Eq. *)
+  (*     symmetry; erewrite add_remove_val_same; eauto. *)
+  (*     now rewrite Sems. *)
+  (* Qed. *)
 
-  Theorem msem_node_relooper:
-    forall G f xss M M' yss,
-      Ordered_nodes G ->
-      msem_node G f xss M M' yss ->
-      forall n, M (S n) ≋ M' n.
-  Proof.
-    induction G as [|node].
-    inversion 2;
-      match goal with Hf: find_node _ [] = _ |- _ => inversion Hf end.
-    intros * Hord Hsem n.
-    assert (Hsem' := Hsem).
-    inversion_clear Hsem' as [???????? Clock Hfind Ins ?? Heqs].
-    pose proof (find_node_not_Is_node_in _ _ _ Hord Hfind) as Hnini.
-    pose proof Hord; inv Hord.
-    pose proof Hfind.
-    simpl in Hfind.
-    destruct (ident_eqb node.(n_name) f) eqn:Hnf.
-    - inv Hfind.
-      eapply msem_equations_cons in Heqs; eauto.
-      eapply msem_eqs_relooper; eauto.
-      apply NoDup_defs_node.
-    - eapply msem_node_cons in Hsem; eauto.
-      now apply ident_eqb_neq.
-  Qed.
+  (* Theorem msem_node_relooper: *)
+  (*   forall G f xss M yss, *)
+  (*     Ordered_nodes G -> *)
+  (*     msem_node G f xss M yss -> *)
+  (*     forall n, M (S n) ≋ n. *)
+  (* Proof. *)
+  (*   induction G as [|node]. *)
+  (*   inversion 2; *)
+  (*     match goal with Hf: find_node _ [] = _ |- _ => inversion Hf end. *)
+  (*   intros * Hord Hsem n. *)
+  (*   assert (Hsem' := Hsem). *)
+  (*   inversion_clear Hsem' as [???????? Clock Hfind Ins ?? Heqs]. *)
+  (*   pose proof (find_node_not_Is_node_in _ _ _ Hord Hfind) as Hnini. *)
+  (*   pose proof Hord; inv Hord. *)
+  (*   pose proof Hfind. *)
+  (*   simpl in Hfind. *)
+  (*   destruct (ident_eqb node.(n_name) f) eqn:Hnf. *)
+  (*   - inv Hfind. *)
+  (*     eapply msem_equations_cons in Heqs; eauto. *)
+  (*     eapply msem_eqs_relooper; eauto. *)
+  (*     apply NoDup_defs_node. *)
+  (*   - eapply msem_node_cons in Hsem; eauto. *)
+  (*     now apply ident_eqb_neq. *)
+  (* Qed. *)
 
   (** The other way around  *)
   Lemma mfby_fby:
-    forall x v0 es M M' xs,
-      mfby x v0 es M M' xs ->
+    forall x v0 es M xs,
+      mfby x v0 es M xs ->
       xs ≈ fby v0 es.
   Proof.
-    intros * (Init & Loop & Spec) n.
+    intros * (Init & Spec) n.
     unfold fby.
     pose proof (Spec n) as Spec'.
     destruct (find_val x (M n)) eqn: Find_n; try contradiction.
     destruct (es n); destruct Spec' as (?& Hx); auto.
     rewrite Hx.
-    clear - Init Loop Spec Find_n.
+    clear - Init Spec Find_n.
     revert dependent v.
     induction n; intros; simpl; try congruence.
     specialize (Spec n).
     destruct (find_val x (M n)); try contradiction.
-    rewrite Loop in Find_n.
     destruct (es n); destruct Spec; try congruence.
     apply IHn; congruence.
   Qed.
 
   Theorem msem_sem_node_equation_reset:
     forall G,
-      (forall f xss M M' yss,
-          msem_node G f xss M M' yss ->
+      (forall f xss M yss,
+          msem_node G f xss M yss ->
           sem_node G f xss yss)
       /\
-      (forall bk H M M' eq,
-          msem_equation G bk H M M' eq ->
+      (forall bk H M eq,
+          msem_equation G bk H M eq ->
           sem_equation G bk H eq).
   Proof.
     intros; apply msem_node_equation_ind;
-      [intros|intros|intros ???????????????????????? Rst|intros|intros];
+      [intros|intros|intros ????????????????????? Rst|intros|intros];
       eauto using sem_equation, mfby_fby, sem_node.
     - econstructor; eauto; intro k; destruct (Rst k) as (?&?&?); intuition.
     - econstructor; auto.
@@ -1712,24 +1680,24 @@ dataflow memory for which the non-standard semantics holds true.
   Qed.
 
   Corollary msem_sem_node:
-    forall G f xss M M' yss,
-      msem_node G f xss M M' yss ->
+    forall G f xss M yss,
+      msem_node G f xss M yss ->
       sem_node G f xss yss.
   Proof.
     intros; eapply (proj1 (msem_sem_node_equation_reset G)); eauto.
   Qed.
 
   Corollary msem_sem_equation:
-    forall G bk H M M' eq,
-      msem_equation G bk H M M' eq ->
+    forall G bk H M eq,
+      msem_equation G bk H M eq ->
       sem_equation G bk H eq.
   Proof.
     intros; eapply (proj2 (msem_sem_node_equation_reset G)); eauto.
   Qed.
 
   Corollary msem_sem_equations:
-    forall G bk H M M' eqs,
-      Forall (msem_equation G bk H M M') eqs ->
+    forall G bk H M eqs,
+      Forall (msem_equation G bk H M) eqs ->
       Forall (sem_equation G bk H) eqs.
   Proof.
     induction 1; constructor; eauto using msem_sem_equation.
